finished exercises or chap 7

Exercises/Chap7.lean
@@ -1,5 +1,7 @@
-namespace Hidden
+import Std.Data.HashMap
 
+-- P1
+namespace Hidden
 def pred (n : Nat) : Nat :=
   match n with 
   | 0 => 0
@@ -43,9 +45,72 @@ theorem zero_sub (n : Nat) : sub 0 n = 0 :=
   Nat.recOn (motive := λ x => sub 0 x = 0) n
     rfl 
     (λ x (ih: sub 0 x = 0) => by simp [sub, ih])
-    
-theorem sub_eq_zero_of_le {m n : Nat} (h : le m n) : m - n = 0 := sorry
-  
-#check Nat.sub_eq_zero_of_le
+end Hidden
 
+-- P2
+namespace Hidden
+def length (l : List α) : Nat :=
+  match l with 
+  | List.nil => 0
+  | List.cons _ t => 1 + length t
+  
+def reverse (l : List α) : List α :=
+  match l with 
+  | List.nil => List.nil
+  | List.cons h t => reverse t ++ (List.cons h List.nil)
+
+theorem length_add (s t : List α) : length (s ++ t) = length s + length t := 
+  List.recOn (motive := λ x => length (x ++ t) = length x + length t) s 
+  (by simp [length])
+  (λ h tail (ih : length (tail ++ t) = length tail + length t) => 
+    by calc
+      length ((List.cons h tail) ++ t) = 1 + length (tail ++ t) := by simp [length]
+      _ = (1 + length tail) + length t := by simp [ih, Nat.add_assoc]
+      _ = length (List.cons h tail) + length t := by simp [length])
+      
+theorem length_reverse (t : List α) : length (reverse t) = length t :=
+  List.recOn (motive := λ x => length (reverse x) = length x) t rfl 
+  (λ hd tl (ih : length (reverse tl) = length tl) => 
+    by calc
+      length (reverse (List.cons hd tl)) = length (reverse tl ++ (List.cons hd List.nil)) := by trivial
+      _ = length (reverse tl) + length (List.cons hd List.nil) := by simp [length_add]
+      _ = length tl + 1 := by simp [ih, length]
+      _ = length (List.cons hd tl) := by simp [length, Nat.add_comm])
+      
+theorem reverse_last (h : α) (l : List α) : reverse (l ++ [h]) = List.cons h (reverse l) := 
+  List.recOn (motive := λ x => reverse (x ++ [h]) = List.cons h (reverse x)) l rfl 
+  (λ hd tl (ih : reverse (tl ++ [h]) = List.cons h (reverse tl)) => by calc
+    reverse ((List.cons hd tl) ++ [h]) = reverse (tl ++ [h]) ++ [hd] := rfl
+    _ = List.cons h (reverse tl) ++ [hd] := by rw [ih]
+    _ = List.cons h (reverse (List.cons hd tl)) := rfl)
+
+theorem reverse_reverse (t : List α) : reverse (reverse t) = t :=
+  List.recOn (motive := λ x => reverse (reverse x) = x) t rfl
+  (λ hd tl (ih : reverse (reverse tl) = tl) => by calc
+    reverse (reverse (List.cons hd tl)) = reverse (reverse tl ++ [hd]) := rfl
+    _ = List.cons hd (reverse (reverse tl)) := by rw [reverse_last]
+    _ = List.cons hd tl := by rw [ih])
+end Hidden
+
+-- P3
+namespace Hidden
+inductive Expr where
+  | const (n : Nat) : Expr
+  | var (v : Nat) : Expr
+  | plus (l r: Expr) : Expr
+  | times (l r : Expr) : Expr
+  
+def eval (e : Expr) (st : Std.HashMap Nat Nat) : Nat :=
+  match e with
+  | Expr.const n => n
+  | Expr.var v => Std.HashMap.find! st v
+  | Expr.plus l r => (eval l st) + (eval r st)
+  | Expr.times l r => (eval l st) * (eval r st)
+  
+open Expr
+def gen_st : Std.HashMap Nat Nat := 
+  let st := Std.HashMap.empty
+  Std.HashMap.insert st 0 5
+
+#eval eval (times (plus (const 3) (var 0)) (times (const 2) (const 2))) gen_st
 end Hidden
